src/Bedrock/Field/Synthesis/New/Signature.v
@@ -111,21 +111,21 @@ Section WithParameters.
 
   Local Notation felem_size_in_words := (felem_size_in_words(FieldRepresentation:=field_representation)).
 
+  (* TODO move these two lemmas to field.v *)
   Lemma FElem_array_truncated_scalar_iff1 px x :
     Lift1Prop.iff1
       (FElem px x)
-      (sep (map:=mem)
-           (emp (map:=mem) (length x = n))
-           (Array.array
+      (Array.array
               (Scalars.truncated_scalar access_size.word)
               (word.of_Z
                  (Z.of_nat (BinIntDef.Z.to_nat (bytes_per_word width))))
-              px (map word.unsigned x))).
+              px (map word.unsigned x)).
   Proof using ok.
-    cbv [FElem Bignum.Bignum field_representation frep].
+    pose proof Types.word_size_in_bytes_pos. 
+    cbv [FElem field_representation frep].
     rewrite Util.array_truncated_scalar_scalar_iff1.
-    Morphisms.f_equiv. Morphisms.f_equiv. Morphisms.f_equiv.
-    destruct Bitwidth.width_cases as [W|W]; rewrite W; trivial.
+    rewrite Z2Nat.id; try lia.
+    split; intros; sepsimpl; try assumption.
   Qed.
 
   Lemma FElemBytes_array_truncated_scalar_iff1 pbs bs :
@@ -282,10 +282,9 @@ Section WithParameters.
            clear; cbn; intuition Lia.lia
     | |- _ = LoadStoreList.list_lengths_from_args _ =>
       autounfold with list_lengths pairs list_lengths;
-      felem_to_array; sepsimpl; rewrite !map_length;
-      repeat match goal with
-             | H : length _ = _ |- _ => rewrite H end;
-      reflexivity
+        felem_to_array; sepsimpl; 
+        rewrite !map_length, !felem_length;
+        reflexivity
     | _ => idtac
     end.
 
@@ -297,9 +296,9 @@ Section WithParameters.
     | H : context [FElem pout ?old_out]
       |- @Lift1Prop.ex1 (list Z) _ _ _ =>
       exists (map word.unsigned old_out)
-    | H : context [Placeholder pout ?old_out ]
+    | H : context [sepclause_of_map (?old_out$@pout)]
       |- @Lift1Prop.ex1 (list Z) _ _ _ =>
-      seprewrite_in Placeholder_iff_FElem_bytes H; extract_ex1_and_emp_in_hyps;
+      unshelve seprewrite_in felem_from_bytes H; [assumption|];
       exists (map word.unsigned (bs2ws (word:=word) (Z.to_nat (bytes_per_word width)) old_out))
     end;
     crush_sep.
@@ -326,7 +325,7 @@ Section WithParameters.
            | |- _ /\ _ => eexists
            end.
 
-    Ltac solve_length x Hlength := rewrite map_length;
+    Ltac solve_length x Hlength := rewrite map_length; rewrite bs2ws_felem_length; [|assumption];
     match goal with
         | H : (FElem _ x * _)%sep _ |- _ => cbv [FElem Bignum.Bignum] in H; sepsimpl_hyps
         | _ => idtac
@@ -336,13 +335,31 @@ Section WithParameters.
         | _ => idtac
     end; rewrite Hlength; auto.
 
+  Lemma map_Z_map_unsigned : forall (x : list word), x = map word.of_Z (map word.unsigned x).
+        intros. rewrite map_map.
+        f_equal; eapply List.nth_error_ext; intros i; rewrite ListUtil.nth_error_map.
+        case (nth_error _ i); cbn; trivial; []; intros; eapply f_equal.
+        symmetry; eapply word.of_Z_unsigned.
+  Qed.
+
+  Lemma map_unsigned_map_Z : forall (x : list byte),
+      map byte.unsigned x = map (word.unsigned (width:=width)) (map word.of_Z (map byte.unsigned x)).
+    intros. rewrite map_map.
+    eapply List.nth_error_ext. intros i. rewrite !ListUtil.nth_error_map.
+    destruct (nth_error _ i) eqn:?; trivial; cbn.
+    apply ListUtil.List.nth_error_In in Heqo. f_equal.
+    rewrite Properties.word.unsigned_of_Z_nowrap; [reflexivity|].
+    pose proof (byte.unsigned_range b).
+    destruct Bitwidth.width_cases as [W|W]; rewrite W; lia.
+Qed.
+
   Section ListBinop.
     Context {res : API.Expr (type_listZ -> type_listZ -> type_listZ)}
             (res_valid :
                valid_func (res (fun _ : API.type => unit)))
             (res_Wf : API.Wf res).
     Context name (bop : BinOp name)
-            (res_eq : forall x y : list word,
+            (res_eq : forall x y : felem,
                 bounded_by bin_xbounds x ->
                 bounded_by bin_ybounds y ->
                 feval (map word.of_Z
@@ -403,26 +420,24 @@ Section WithParameters.
         {
           (* lists_reserved_with_initial_context *)
           lists_reserved_simplify pout; try solve_equivalence_side_conditions;
-          try solve_length (bs2ws (word:=word) (Z.to_nat (bytes_per_word width)) out) outbounds_length.
+          try solve_length out outbounds_length.
         } }
-      { postcondition_simplify; [ | | ]; cycle -1.
-        { refine (proj1 (Proper_sep_iff1 _ _ _ _ _ _ _) _);
+      { unshelve postcondition_simplify; [ | | | ].
+        { refine (exist _ x3 _); (* TODO move to a definition/lemma? *) 
+          abstract (erewrite <- map_length; rewrite H10; 
+          erewrite length_list_Z_bounded_by; eauto using res_bounds; apply repeat_length). }
+        3: { refine (proj1 (Proper_sep_iff1 _ _ _ _ _ _ _) _);
             [symmetry; eapply FElem_array_truncated_scalar_iff1 | reflexivity | sepsimpl ].
-          2:eassumption.
-          erewrite <-map_length.
-          match goal with H : map word.unsigned _ = API.interp (res _) _ _ |- _ =>
-            rewrite H end.
-          erewrite length_list_Z_bounded_by; eauto using res_bounds; apply repeat_length. }
+            cbv [felem_to_list proj1_sig].
+          eassumption. (* I think this means my bytes pre dance in field.v is not necessary*) }
         { (* output correctness *)
           erewrite <-res_eq; auto.
+          f_equal. unfold felem_to_list at 1. cbv [proj1_sig].
           match goal with H : map word.unsigned _ = API.interp (res _) _ _ |- _ =>
             rewrite <-H end.
-          rewrite map_map.
-          f_equal; eapply List.nth_error_ext; intros i; rewrite ListUtil.nth_error_map.
-          case (nth_error _ i); cbn; trivial; []; intros; eapply f_equal.
-          symmetry; eapply word.of_Z_unsigned. }
+          apply map_Z_map_unsigned. }
         { (* output bounds *)
-          cbn [bounded_by field_representation frep] in *.
+          cbn [bounded_by field_representation frep proj1_sig felem_to_list] in *.
           match goal with H : map word.unsigned _ = API.interp (res _) _ _ |- _ =>
             rewrite H end.
           eauto using res_bounds. } }
@@ -435,7 +450,7 @@ Section WithParameters.
                valid_func (res (fun _ : API.type => unit)))
             (res_Wf : API.Wf res).
     Context name (uop : UnOp name)
-            (res_eq : forall x : list word,
+            (res_eq : forall x : felem,
                 bounded_by un_xbounds x ->
                 feval (map word.of_Z
                            (API.interp (res _) (map word.unsigned x)))
@@ -490,29 +505,28 @@ Section WithParameters.
         { (* lists_reserved_with_initial_context *)
           lists_reserved_simplify pout.
           all: try solve_equivalence_side_conditions.
-          solve_length (bs2ws (word:=word) (Z.to_nat (bytes_per_word width)) out) outbounds_length. } }
-      { postcondition_simplify; [ | | ].
+          solve_length out outbounds_length. } }
+      { unshelve postcondition_simplify; [ | | | ].
+        { refine (exist _ x2 _). (* TODO move to a definition/lemma? *) 
+          abstract (erewrite <- map_length; rewrite H8; 
+          erewrite length_list_Z_bounded_by; eauto using res_bounds; apply repeat_length). }
         { (* output correctness *)
-          eapply res_eq; auto. }
+          rewrite <- res_eq; [|assumption]. 
+          f_equal. unfold felem_to_list at 1. cbv [proj1_sig]. 
+          match goal with H : map word.unsigned _ = expr.interp _ (res _) _ |- _ =>
+            rewrite <-H end.
+          apply map_Z_map_unsigned. } 
         { (* output bounds *)
-          cbn [bounded_by field_representation frep] in *.
-          erewrite Util.map_unsigned_of_Z, MaxBounds.map_word_wrap_bounded
-            by eauto using relax_list_Z_bounded_by.
-          eauto. }
+          cbn [bounded_by field_representation frep proj1_sig felem_to_list] in *.
+          match goal with H : map word.unsigned _ = _ |- _ =>
+            rewrite H end.
+          eauto using res_bounds. }
         { (* separation-logic postcondition *)
           eapply Proper_sep_iff1;
             [ solve [apply FElem_array_truncated_scalar_iff1]
             | reflexivity | ].
-          sepsimpl; [ | ].
-          { rewrite !map_length. apply outbounds_length; auto. }
-          { erewrite Util.map_unsigned_of_Z, MaxBounds.map_word_wrap_bounded
-              by eauto using relax_list_Z_bounded_by.
-            rewrite MakeAccessSizes.bytes_per_word_eq.
-            clear outbounds_length; subst.
-            match goal with
-              H : map word.unsigned _ = API.interp (res _) _ |- _ =>
-              rewrite <-H end.
-            auto. } } }
+           cbv [felem_to_list proj1_sig]. assumption. }
+      }
     Qed.
   End ListUnop.
 
@@ -575,32 +589,27 @@ Section WithParameters.
           symmetry.
           erewrite length_list_Z_bounded_by; [| eapply tight_bounds_tighter_than_max, res_bounds].
           cbv [max_bounds]. rewrite repeat_length. rewrite map_length.
-          cbv [FElem Bignum.Bignum] in *. sepsimpl. auto.
+          rewrite bs2ws_felem_length; auto.
         } }
-      { postcondition_simplify; [ | | ].
+      { unshelve postcondition_simplify; [ | | | ].
+        { refine (exist _ x1 _). (* TODO move to a definition/lemma? *) 
+          abstract (erewrite <- map_length; rewrite H6; 
+          erewrite length_list_Z_bounded_by; eauto using res_bounds; apply repeat_length). }
         { (* output correctness *)
-          eapply res_eq; auto. }
+          erewrite <- res_eq. f_equal. cbv [felem_to_list proj1_sig].
+          match goal with H : map word.unsigned _ = API.interp (res _) _ |- _ =>
+            rewrite <-H end.
+          apply map_Z_map_unsigned. }
         { (* output bounds *)
-          cbn [bounded_by field_representation frep] in *.
-          erewrite Util.map_unsigned_of_Z, MaxBounds.map_word_wrap_bounded
-            by eauto using relax_list_Z_bounded_by. cbv [Field.tight_bounds]. simpl.
-          eauto. }
+          cbn [bounded_by field_representation frep proj1_sig felem_to_list] in *.
+          match goal with H : map word.unsigned _ = _ |- _ =>
+            rewrite H end.
+          eauto using res_bounds. }
         { (* separation-logic postcondition *)
           eapply Proper_sep_iff1;
             [ solve [apply FElem_array_truncated_scalar_iff1]
             | reflexivity | ].
-          sepsimpl; [ | ].
-          { rewrite !map_length.
-            erewrite length_list_Z_bounded_by; [| eapply tight_bounds_tighter_than_max, res_bounds].
-            cbv [max_bounds]; rewrite repeat_length; trivial. }
-          { erewrite Util.map_unsigned_of_Z, MaxBounds.map_word_wrap_bounded
-              by eauto using relax_list_Z_bounded_by.
-            rewrite MakeAccessSizes.bytes_per_word_eq.
-            (* clear tight_bounds_length; subst. *)
-            match goal with
-              H : map word.unsigned _ = API.interp (res _) _ |- _ =>
-              rewrite <-H end.
-            auto. } } }
+          cbv [felem_to_list proj1_sig]. assumption. } }
     Qed.
   End FromWord.
 
@@ -663,8 +672,9 @@ Section WithParameters.
           cbn [type.app_curried fst snd].
           apply res_bounds.
           rewrite max_bounds_range_iff.
+
           seprewrite_in @FElem_array_truncated_scalar_iff1 H1; extract_ex1_and_emp_in H1.
-          ssplit; rewrite ?map_length; trivial.
+          ssplit; rewrite ?map_length, ?felem_length; trivial.
           eapply List.Forall_map, Forall_forall; intros.
           rewrite MakeAccessSizes.bits_per_word_eq_width.
           eapply Properties.word.unsigned_range. }
@@ -673,12 +683,16 @@ Section WithParameters.
           all:try solve_equivalence_side_conditions;
           seprewrite_in (FElem_array_truncated_scalar_iff1 pout) H1; extract_ex1_and_emp_in H1; try eassumption.
           seprewrite_in (FElem_array_truncated_scalar_iff1 px) H1; extract_ex1_and_emp_in H1.
-          setoid_rewrite max_bounds_range_iff in res_bounds.
-          rewrite (fun x pf => proj1 (res_bounds x pf)), ?map_length; trivial.
-          ssplit; rewrite ?map_length; trivial.
-          eapply List.Forall_map, Forall_forall; intros.
-          rewrite MakeAccessSizes.bits_per_word_eq_width.
-          eapply Properties.word.unsigned_range. } }
+
+          (* woah that's repetetive, fix *)
+          rewrite map_length. rewrite bs2ws_felem_length; auto.
+          erewrite length_list_Z_bounded_by.
+          2: { apply res_bounds. erewrite max_bounds_range_iff.
+          ssplit; rewrite ?map_length, ?felem_length; auto.
+          eapply List.Forall_map, Forall_forall; intros;
+          rewrite MakeAccessSizes.bits_per_word_eq_width;
+          eapply Properties.word.unsigned_range. }
+          cbv [max_bounds]; rewrite repeat_length; trivial. }}
       postcondition_simplify.
       eapply sep_assoc,sep_comm, sep_assoc. eapply Proper_sep_iff1.
       { eapply FElem_array_truncated_scalar_iff1. }
@@ -688,11 +702,12 @@ Section WithParameters.
         try (use_sep_assumption; cancel; cbv [seps]);
         seprewrite_in (FElem_array_truncated_scalar_iff1 px) H1; extract_ex1_and_emp_in H1; trivial.
       Morphisms.f_equiv.
-      rewrite H5.
-      rewrite <-(res_eq x) at 2 by trivial.
+      rewrite H6.
+      rewrite <-(res_eq x) at 2.
       rewrite Util.map_unsigned_of_Z.
       erewrite map_word_wrap_bounded; trivial.
       eapply max_bounds_range_iff; ssplit; eauto.
+      rewrite felem_length. trivial.
     Qed.
   End FelemCopy.
 
@@ -784,40 +799,42 @@ Section WithParameters.
       autounfold with equivalence pairs;
       rewrite <-?MakeAccessSizes.bytes_per_word_eq;
       sepsimpl; crush_sep; try solve [solve_equivalence_side_conditions].
+        2: {
         change (Z.of_nat (bytes_per access_size.one)) with 1.
          try
           erewrite Util.map_unsigned_of_Z, map_word_wrap_bounded.
           { rewrite <-(ByteBounds.byte_map_of_Z_unsigned bs) in H.
             seprewrite_in (symmetry! @Util.array_truncated_scalar_ptsto_iff1) H.
             ecancel_assumption. }
-          { eapply byte_unsigned_within_max_bounds; try rewrite byte_bounds_length; trivial. }
+          { eapply byte_unsigned_within_max_bounds; try rewrite byte_bounds_length; trivial. } }
+        { auto using map_unsigned_map_Z. }
         { (* lists_reserved_with_initial_context *)
           lists_reserved_simplify pout.
           all: try solve_equivalence_side_conditions.
-          solve_length (bs2ws (word:=word) (Z.to_nat (bytes_per_word width)) out) tight_bounds_length.
+          solve_length out tight_bounds_length.
         } }
-      { postcondition_simplify; [ | | ].
+      { unshelve postcondition_simplify; [ | | | ].
+        { refine (exist _ (x1) _).
+          erewrite <-map_length. rewrite H8.
+          apply tight_bounds_length; auto. }
         { (* output correctness *)
-          eapply res_eq; auto. }
+          erewrite <- res_eq. f_equal. cbv [felem_to_list proj1_sig].
+          match goal with H : map word.unsigned _ = API.interp (res _) _ |- _ =>
+            rewrite <-H end.
+          apply map_Z_map_unsigned.
+          assumption. }
         { (* output bounds *)
-          cbn [bounded_by field_representation frep] in *.
-          erewrite Util.map_unsigned_of_Z, MaxBounds.map_word_wrap_bounded
-            by eauto using relax_list_Z_bounded_by.
-          eauto. }
+          cbn [bounded_by field_representation frep proj1_sig felem_to_list] in *.
+          match goal with H : map word.unsigned _ = API.interp (res _) _ |- _ =>
+            rewrite H end.
+          apply res_bounds. assumption. }
         { (* separation-logic postcondition *)
           eapply Proper_sep_iff1;
             [ solve [apply FElem_array_truncated_scalar_iff1]
-            | reflexivity | ].
-          sepsimpl; [ | ].
-          { rewrite !map_length; apply tight_bounds_length; auto. }
-          { erewrite Util.map_unsigned_of_Z, MaxBounds.map_word_wrap_bounded
-              by eauto using relax_list_Z_bounded_by.
+            | reflexivity | cbv [felem_to_list proj1_sig] ].
             rewrite MakeAccessSizes.bytes_per_word_eq.
             clear tight_bounds_length; subst.
-            match goal with
-              H : map word.unsigned _ = API.interp (res _) _ |- _ =>
-              rewrite <-H end.
-            auto. } } }
+            auto. } }
     Qed.
   End FromBytes.
 
@@ -1020,7 +1037,7 @@ Context
 
     Lemma FElem_max_bounds : forall px x m R, (FElem px x * R)%sep m -> list_Z_bounded_by (@max_bounds width n) (map word.unsigned x).
     Proof.
-      intros. eapply max_bounds_words. cbv [FElem Bignum.Bignum] in H. sepsimpl. eauto.
+      intros. eapply max_bounds_words. rewrite felem_length. eauto.
     Qed.
 
     Lemma select_znz_correct f :
@@ -1034,8 +1051,8 @@ Context
       cbv [list_selectznz_insizes list_selectznz_outsizes list_selectznz_inlengths].
       cbv beta; intros; subst f. cbv [make_bedrock_func] in *.
       cleanup.
-      pose proof (FElem_max_bounds _ _ _ _ H1) as Hxbounds.
-      pose proof (FElem_max_bounds _ _ _ _ H2) as Hybounds.
+      pose proof (FElem_max_bounds _ _ _ _ H2) as Hxbounds.
+      pose proof (FElem_max_bounds _ _ _ _ H3) as Hybounds.
       match goal with
       | H : ZRange.is_bounded_by_bool _ _ = _ |- _ => rename H into Hbound
       | _ => idtac
@@ -1067,7 +1084,7 @@ Context
             lists_reserved_simplify pout.
             all: try solve_equivalence_side_conditions.
             destruct (bit_range_eq _ Hbound) as [Hbit| Hbit]; rewrite Hbit; simpl; auto; cbv [FElem Bignum.Bignum] in *; sepsimpl;
-            repeat rewrite map_length;
+            repeat rewrite map_length, ?bs2ws_felem_length, ?felem_length;
             match goal with
               | H : ?n1 = _ |- ?n1 = _ => rewrite H
               | _ => idtac
@@ -1078,27 +1095,21 @@ Context
             - rewrite Hbit. simpl. eapply Proper_sep_iff1.
                 + apply FElem_array_truncated_scalar_iff1.
                 + intros; split; intros; eauto.
-                + sepsimpl; try ecancel_assumption.
-                    * erewrite <- map_length. erewrite length_list_Z_bounded_by; eauto.
-                      cbv [max_bounds]. rewrite repeat_length. eauto.
-                    * specialize (res_eq x y pc); rewrite Hbit in res_eq; simpl in res_eq.
-                      erewrite <- res_eq; eauto; rewrite <- Hbit; simpl in *; eauto.
-                      match goal with
-                      | H : map word.unsigned _ = _ |- _ => rewrite <- H
-                      | _ => idtac
-                      end; eauto.
+                + specialize (res_eq x y pc); rewrite Hbit in res_eq; simpl in res_eq.
+                  erewrite <- res_eq; eauto; rewrite <- Hbit; simpl in *; eauto.
+                  match goal with
+                  | H : map word.unsigned _ = _ |- _ => rewrite <- H
+                  | _ => idtac
+                  end; eauto.
             - rewrite Hbit; simpl; eapply Proper_sep_iff1.
                 + apply FElem_array_truncated_scalar_iff1.
                 + intros; split; intros; eauto.
-                + sepsimpl; try ecancel_assumption.
-                    * erewrite <- map_length; erewrite length_list_Z_bounded_by; eauto;
-                      cbv [max_bounds]; rewrite repeat_length; eauto.
-                    * specialize (res_eq x y pc); rewrite Hbit in res_eq; simpl in res_eq.
-                      erewrite <- res_eq; eauto; rewrite <- Hbit; simpl in *; eauto.
-                      match goal with
-                      | H : map word.unsigned _ = _ |- _ => rewrite <- H
-                      | _ => idtac
-                      end; eauto.
+                + specialize (res_eq x y pc); rewrite Hbit in res_eq; simpl in res_eq.
+                  erewrite <- res_eq; eauto; rewrite <- Hbit; simpl in *; eauto.
+                  match goal with
+                  | H : map word.unsigned _ = _ |- _ => rewrite <- H
+                  | _ => idtac
+                  end; eauto.
     Qed.
   End SelectZnZ.
 End WithParameters.
